Modification in formatting

Sequences/SeqOfSeq.dfy
@@ -6,101 +6,101 @@ module SeqOfSeq {
 
   /*concatenates a sequence of sequences into a single sequence. Works by adding 
   elements in order from first to last */
-  function method concat<T>(s: seq<seq<T>>): seq<T>
+  function method flatten<T>(s: seq<seq<T>>): seq<T>
   decreases |s|
   {
     if |s| == 0 then []
-    else s[0] + concat(s[1..])
+    else s[0] + flatten(s[1..])
   }
 
   /* concatenating two sequences of sequences is equivalent to concatenating 
   each sequence of sequences seperately, and then concatenating the two resulting 
   sequences together */
-  lemma lemma_concat_adds<T>(a: seq<seq<T>>, b: seq<seq<T>>)
-    ensures concat(a + b) == concat(a) + concat(b)
+  lemma lemma_flatten_concat<T>(a: seq<seq<T>>, b: seq<seq<T>>)
+    ensures flatten(a + b) == flatten(a) + flatten(b)
   {
     if |a| == 0 {
       assert a + b == b;
     } else {
       calc == {
-        concat(a + b);
+        flatten(a + b);
           { assert (a + b)[0] == a[0];  assert (a + b)[1..] == a[1..] + b; }
-        a[0] + concat(a[1..] + b);
-        a[0] + concat(a[1..]) + concat(b);
-        concat(a) + concat(b);
+        a[0] + flatten(a[1..] + b);
+        a[0] + flatten(a[1..]) + flatten(b);
+        flatten(a) + flatten(b);
       }
     }
   }
 
-  /* concatenates the sequence of sequences into a single sequence. Works by adding 
+  /* concatenates the sequence of sequences into a single sequence. Works by concatenating 
   elements from last to first */
-  function method concat_reverse<T>(s: seq<seq<T>>): seq<T>
+  function method flatten_reverse<T>(s: seq<seq<T>>): seq<T>
   decreases |s|
   {
     if |s| == 0 then []
-    else concat_reverse(drop_last(s)) + last(s)
+    else flatten_reverse(drop_last(s)) + last(s)
   }
 
   /* concatenating two reversed sequences of sequences is the same as reversing two 
-  sequences of sequences and then adding the two resulting sequences together */
-  lemma lemma_concat_reverse_adds<T>(A:seq<seq<T>>, B:seq<seq<T>>)
-  ensures concat_reverse(A + B) == concat_reverse(A) + concat_reverse(B)
+  sequences of sequences and then concattenating the two resulting sequences together */
+  lemma lemma_flatten_reverse_concat<T>(A:seq<seq<T>>, B:seq<seq<T>>)
+  ensures flatten_reverse(A + B) == flatten_reverse(A) + flatten_reverse(B)
   {
     if |B| == 0 {
-      assert concat_reverse(B) == [];
+      assert flatten_reverse(B) == [];
       assert A+B == A;
     } else {
       calc == {
-        concat_reverse(A + B);
+        flatten_reverse(A + B);
           { assert last(A + B) == last(B);  assert drop_last(A + B) == A + drop_last(B); }
-        concat_reverse(A + drop_last(B)) + last(B);
-        concat_reverse(A) + concat_reverse(drop_last(B)) + last(B);
-        concat_reverse(A) + concat_reverse(B);
+        flatten_reverse(A + drop_last(B)) + last(B);
+        flatten_reverse(A) + flatten_reverse(drop_last(B)) + last(B);
+        flatten_reverse(A) + flatten_reverse(B);
       }
     }
   }
 
   /* both methods of concatenating sequence (starting from front v. starting from back)
   result in the same sequence */
-  lemma lemma_concat_and_concat_reverse_are_equivalent<T>(s: seq<seq<T>>)
-    ensures concat(s) == concat_reverse(s)
+  lemma lemma_flatten_and_flatten_reverse_are_equivalent<T>(s: seq<seq<T>>)
+    ensures flatten(s) == flatten_reverse(s)
   {
     if |s| == 0 {
     } else {
       calc == {
-        concat_reverse(s);
-        concat_reverse(drop_last(s)) + last(s);
-          { lemma_concat_and_concat_reverse_are_equivalent(drop_last(s)); }
-        concat(drop_last(s)) + last(s);
-        concat(drop_last(s)) + concat([last(s)]);
-          { lemma_concat_adds(drop_last(s), [last(s)]); 
+        flatten_reverse(s);
+        flatten_reverse(drop_last(s)) + last(s);
+          { lemma_flatten_and_flatten_reverse_are_equivalent(drop_last(s)); }
+        flatten(drop_last(s)) + last(s);
+        flatten(drop_last(s)) + flatten([last(s)]);
+          { lemma_flatten_concat(drop_last(s), [last(s)]); 
         assert s == drop_last(s) + [last(s)]; }
-        concat(s);
+        flatten(s);
       }
     }
   }
 
   /* the concatenated sequence's length is greater than or equal to each individual
   inner sequence's length */
-  lemma lemma_concat_length_ge_single_element_length<T>(s: seq<seq<T>>, i: int)
+  lemma lemma_flatten_length_ge_single_element_length<T>(s: seq<seq<T>>, i: int)
     requires 0 <= i < |s|
-    ensures |concat_reverse(s)| >= |s[i]|
+    ensures |flatten_reverse(s)| >= |s[i]|
   {
     if i < |s| - 1 {
-      lemma_concat_length_ge_single_element_length(s[..|s|-1], i);
+      lemma_flatten_length_ge_single_element_length(s[..|s|-1], i);
     }
   }
 
   /* the length of concatenating sequence in a sequence together will be no longer 
   than the length of the original sequence of sequences multiplied by the length of 
   the longest sequence */
-  lemma lemma_concat_length_le_mul<T>(s: seq<seq<T>>, j: int)
+  lemma lemma_flatten_length_le_mul<T>(s: seq<seq<T>>, j: int)
     requires forall i | 0 <= i < |s| :: |s[i]| <= j
-    ensures |concat_reverse(s)| <= |s| * j
+    ensures |flatten_reverse(s)| <= |s| * j
   {
     if |s| == 0 {
     } else {
-      lemma_concat_length_le_mul(s[..|s|-1], j);
+      lemma_flatten_length_le_mul(s[..|s|-1], j);
     }
   }
 
