Sequences/SeqExtrema.dfy
@@ -6,7 +6,7 @@ module SeqExtrema {
   import opened SeqLast
   import Math = Mathematics
 
-  /* returns the maximum integer value in the sequence */
+  /* finds the maximum integer value in the sequence */
   function method {:opaque} max(s: seq<int>): int
     requires 0 < |s|
     ensures forall k :: k in s ==> max(s) >= k
@@ -30,7 +30,7 @@ module SeqExtrema {
     }
   }
 
-  /* returns the minimum integer value in the sequence */
+  /* finds the minimum integer value in the sequence */
   function method {:opaque} min(s: seq<int>): int
     requires 0 < |s|
     ensures forall k :: k in s ==> min(s) <= k
@@ -54,23 +54,6 @@ module SeqExtrema {
     }
   }
 
-  /* the maximum value in sequence 1 is greater than or equal to the maximum
-  value of sequence 2 */
-  lemma lemma_max_correspondence(s1:seq<int>, s2:seq<int>, wit: seq<nat>)
-    requires 0 < |s1|
-    requires 0 < |s2|
-    requires |wit| == |s2|
-    requires forall j:nat :: j < |wit| ==> wit[j] < |s1|
-    requires forall i :: 0 <= i < |s2| ==> s2[i] <= s1[wit[i]]
-    ensures max(s2) <= max(s1)
-  {
-    if max(s2) > max(s1) {
-      var k :| 0 <= k < |s2| && s2[k] == max(s2);
-      assert s1[wit[k]] in s1;
-      assert false;
-    }
-  }
-
   /* the maximum element in any subsequence will not be greater than the maximum element in 
   the full sequence */
   lemma lemma_subseq_max(s: seq<int>, from: nat, to: nat)
@@ -78,20 +61,10 @@ module SeqExtrema {
     ensures max(s[from .. to]) <= max(s)
   {
     var subseq := s[from .. to];
-    lemma_max_correspondence(s, subseq, seq(|subseq|, i requires 0<=i<|subseq| => i + from));
-  }
-
-  lemma lemma_min_correspondence(s1:seq<int>, s2:seq<int>, wit: seq<nat>)
-    requires 0 < |s1|
-    requires 0 < |s2|
-    requires |wit| == |s2|
-    requires forall j:nat :: j < |wit| ==> wit[j] < |s1|
-    requires forall i :: 0 <= i < |s2| ==> s2[i] >= s1[wit[i]]
-    ensures min(s2) >= min(s1)
-  {
-    if min(s2) < min(s1) {
-      var k :| 0 <= k < |s2| && s2[k] == min(s2);
-      assert s1[wit[k]] in s1;
+    if max(subseq) > max(s) {
+      var k :| 0 <= k < |subseq| && subseq[k] == max(subseq);
+      assert s[seq(|subseq|, i requires 0 <= i < |subseq| => i + from)[k]] in s;
+      assert false;
     }
   }
 
@@ -100,7 +73,10 @@ module SeqExtrema {
     ensures min(s[from..to]) >= min(s)
   {
     var subseq := s[from..to];
-    lemma_min_correspondence(s, subseq, seq(|subseq|, i requires 0<=i<|subseq| => i + from));
+    if min(subseq) < min (s) {
+      var k :| 0 <= k < |subseq| && subseq[k] == min(subseq);
+      assert s[seq(|subseq|, i requires 0<=i<|subseq| => i + from)[k]] in s;
+    }
   }
 
 }
